src/SimpleA64InsSem.v
@@ -162,87 +162,87 @@ Module AArch64 <: InsSemSig.
            trigger (RegEWrite (full_reg_of_reg (GPR dst)) res)
       end.
 
-  Definition decode_reg (b4 b3 b2 b1 b0 : bool) : option gpr :=
-    List.nth_error
-      [R0; R1; R2; R3; R4; R5; R6; R7; R8; R9]
-      (wordToNat (WS b0 (WS b1 (WS b2 (WS b3 (WS b4 WO)))))).
+  Section Decode.
+    Definition decode_reg (b4 b3 b2 b1 b0 : bool) : option gpr :=
+      List.nth_error
+        [R0; R1; R2; R3; R4; R5; R6; R7; R8; R9]
+        (wordToNat (WS b0 (WS b1 (WS b2 (WS b3 (WS b4 WO)))))).
 
-  Definition decode_log_op (b1 b0 : bool) : option log_op :=
-    match b1, b0 with
-    | false, false => Some LOAnd
-    | false, true => Some LOOr
-    | true, false => Some LOXor
-    | _, _ => None
-    end.
+    Definition decode_log_op (b1 b0 : bool) : option log_op :=
+      match b1, b0 with
+      | false, false => Some LOAnd
+      | false, true => Some LOOr
+      | true, false => Some LOXor
+      | _, _ => None
+      end.
 
-  Notation "w '~' b" := (WS b w) (at level 7, left associativity, format "w '~' b") : word_scope.
+    Notation "w '~' b" := (WS b w) (at level 7, left associativity, format "w '~' b") : word_scope.
 
-  Definition decode (machine_code : mem_slc_val) : option ast :=
-    match reg_val_of_mem_slc_val 32 machine_code with
-    (* LDR (register) 64-bit, LSL-0:
+    Definition decode (machine_code : mem_slc_val) : option ast :=
+      match reg_val_of_mem_slc_val 32 machine_code with
+      (* LDR (register) 64-bit, LSL-0:
        [1(x=1) 111 0 00 01 1 Rm (option=011) (S=0) 10 Rn Rt] *)
-    | (WO~ 1~1 ~ 1~1~1 ~ 0 ~ 0~0 ~ 0~1 ~ 1 ~ Rm4~Rm3~Rm2~Rm1~Rm0 ~ 0~1~1 ~ 0
-         ~ 1~0 ~ Rn4~Rn3~Rn2~Rn1~Rn0 ~ Rt4~Rt3~Rt2~Rt1~Rt0)%word =>
-      match decode_reg Rm4 Rm3 Rm2 Rm1 Rm0,
-            decode_reg Rn4 Rn3 Rn2 Rn1 Rn0,
-            decode_reg Rt4 Rt3 Rt2 Rt1 Rt0 with
-      | Some Rm, Some Rn, Some Rt => Some (Load Rt Rn (OpGPR Rm))
-      | _, _, _ => None
-      end
-    (* LDR (immediate) unsigned offset, 64-bit:
+      | (WO~ 1~1 ~ 1~1~1 ~ 0 ~ 0~0 ~ 0~1 ~ 1 ~ Rm4~Rm3~Rm2~Rm1~Rm0 ~ 0~1~1 ~ 0
+           ~ 1~0 ~ Rn4~Rn3~Rn2~Rn1~Rn0 ~ Rt4~Rt3~Rt2~Rt1~Rt0)%word =>
+        match decode_reg Rm4 Rm3 Rm2 Rm1 Rm0,
+              decode_reg Rn4 Rn3 Rn2 Rn1 Rn0,
+              decode_reg Rt4 Rt3 Rt2 Rt1 Rt0 with
+        | Some Rm, Some Rn, Some Rt => Some (Load Rt Rn (OpGPR Rm))
+        | _, _, _ => None
+        end
+      (* LDR (immediate) unsigned offset, 64-bit:
        [1(x=1) 111 0 01 01 imm12 Rn Rt] *)
-    | (WO~ 1~1 ~ 1~1~1 ~ 0 ~ 0~1 ~ 0~1 ~ i11~i10~i9~i8~i7~i6~i5~i4~i3~i2~i1~i0
-         ~ Rn4~Rn3~Rn2~Rn1~Rn0 ~ Rt4~Rt3~Rt2~Rt1~Rt0)%word =>
-      match decode_reg Rn4 Rn3 Rn2 Rn1 Rn0,
-            decode_reg Rt4 Rt3 Rt2 Rt1 Rt0 with
-      | Some Rn, Some Rt =>
-        let imm12 := WS i0 (WS i1 (WS i2 (WS i3 (WS i4 (WS i5 (WS i6 (WS i7
-                     (WS i8 (WS i9 (WS i10 (WS i11 WO))))))))))) in
-        let offset := wordToNat (imm12 ^<< 3) in
-        Some (Load Rt Rn (OpImm offset))
-      | _, _ => None
-      end
-    (* STR (register) 64-bit, LSL-0:
+      | (WO~ 1~1 ~ 1~1~1 ~ 0 ~ 0~1 ~ 0~1 ~ i11~i10~i9~i8~i7~i6~i5~i4~i3~i2~i1~i0
+           ~ Rn4~Rn3~Rn2~Rn1~Rn0 ~ Rt4~Rt3~Rt2~Rt1~Rt0)%word =>
+        match decode_reg Rn4 Rn3 Rn2 Rn1 Rn0,
+              decode_reg Rt4 Rt3 Rt2 Rt1 Rt0 with
+        | Some Rn, Some Rt =>
+          let imm12 := WS i0 (WS i1 (WS i2 (WS i3 (WS i4 (WS i5 (WS i6 (WS i7
+                                                                           (WS i8 (WS i9 (WS i10 (WS i11 WO))))))))))) in
+          let offset := wordToNat (imm12 ^<< 3) in
+          Some (Load Rt Rn (OpImm offset))
+        | _, _ => None
+        end
+      (* STR (register) 64-bit, LSL-0:
        [1(x=1) 111 0 00 00 1 Rm (option=011) (S=0) 10 Rn Rt] *)
-    | (WO~ 1~1 ~ 1~1~1 ~ 0 ~ 0~0 ~ 0~0 ~ 1 ~ Rm4~Rm3~Rm2~Rm1~Rm0 ~ 0~1~1 ~ 0
-         ~ 1~0 ~ Rn4~Rn3~Rn2~Rn1~Rn0 ~ Rt4~Rt3~Rt2~Rt1~Rt0)%word =>
-      match decode_reg Rm4 Rm3 Rm2 Rm1 Rm0,
-            decode_reg Rn4 Rn3 Rn2 Rn1 Rn0,
-            decode_reg Rt4 Rt3 Rt2 Rt1 Rt0 with
-      | Some Rm, Some Rn, Some Rt => Some (Store (OpGPR Rt) Rn (OpGPR Rm))
-      | _, _, _ => None
-      end
-    (* STR (immediate) unsigned offset, 64-bit:
+      | (WO~ 1~1 ~ 1~1~1 ~ 0 ~ 0~0 ~ 0~0 ~ 1 ~ Rm4~Rm3~Rm2~Rm1~Rm0 ~ 0~1~1 ~ 0
+           ~ 1~0 ~ Rn4~Rn3~Rn2~Rn1~Rn0 ~ Rt4~Rt3~Rt2~Rt1~Rt0)%word =>
+        match decode_reg Rm4 Rm3 Rm2 Rm1 Rm0,
+              decode_reg Rn4 Rn3 Rn2 Rn1 Rn0,
+              decode_reg Rt4 Rt3 Rt2 Rt1 Rt0 with
+        | Some Rm, Some Rn, Some Rt => Some (Store (OpGPR Rt) Rn (OpGPR Rm))
+        | _, _, _ => None
+        end
+      (* STR (immediate) unsigned offset, 64-bit:
        [1(x=1) 111 0 01 00 imm12 Rn Rt] *)
-    | (WO~ 1~1 ~ 1~1~1 ~ 0 ~ 0~1 ~ 0~0 ~ i11~i10~i9~i8~i7~i6~i5~i4~i3~i2~i1~i0
-         ~ Rn4~Rn3~Rn2~Rn1~Rn0 ~ Rt4~Rt3~Rt2~Rt1~Rt0)%word =>
-      match decode_reg Rn4 Rn3 Rn2 Rn1 Rn0,
-            decode_reg Rt4 Rt3 Rt2 Rt1 Rt0 with
-      | Some Rn, Some Rt =>
-        let imm12 := WS i0 (WS i1 (WS i2 (WS i3 (WS i4 (WS i5 (WS i6 (WS i7
-                     (WS i8 (WS i9 (WS i10 (WS i11 WO))))))))))) in
-        let offset := wordToNat (imm12 ^<< 3) in
-        Some (Store (OpGPR Rt) Rn (OpImm offset))
-      | _, _ => None
-      end
-    (* AND/EOR/ORR (shifted register), 64-bit, LSL-0:
+      | (WO~ 1~1 ~ 1~1~1 ~ 0 ~ 0~1 ~ 0~0 ~ i11~i10~i9~i8~i7~i6~i5~i4~i3~i2~i1~i0
+           ~ Rn4~Rn3~Rn2~Rn1~Rn0 ~ Rt4~Rt3~Rt2~Rt1~Rt0)%word =>
+        match decode_reg Rn4 Rn3 Rn2 Rn1 Rn0,
+              decode_reg Rt4 Rt3 Rt2 Rt1 Rt0 with
+        | Some Rn, Some Rt =>
+          let imm12 := WS i0 (WS i1 (WS i2 (WS i3 (WS i4 (WS i5 (WS i6 (WS i7
+                                                                           (WS i8 (WS i9 (WS i10 (WS i11 WO))))))))))) in
+          let offset := wordToNat (imm12 ^<< 3) in
+          Some (Store (OpGPR Rt) Rn (OpImm offset))
+        | _, _ => None
+        end
+      (* AND/EOR/ORR (shifted register), 64-bit, LSL-0:
        [(sf=1) opc 01010 (shift=00) (N=0) Rm (imm6=000000) Rn Rd] *)
-    | (WO~ opc1~opc0 ~ 0~1~0~1~0 ~ 0~0 ~ 0 ~ Rm4~Rm3~Rm2~Rm1~Rm0 ~ 0~0~0~0~0~0
-         ~ Rn4~Rn3~Rn2~Rn1~Rn0 ~ Rd4~Rd3~Rd2~Rd1~Rd0)%word =>
-      match decode_log_op opc1 opc0,
-            decode_reg Rm4 Rm3 Rm2 Rm1 Rm0,
-            decode_reg Rn4 Rn3 Rn2 Rn1 Rn0,
-            decode_reg Rd4 Rd3 Rd2 Rd1 Rd0 with
-      | Some op, Some Rm, Some Rn, Some Rd => Some (LogOp op Rd Rn (OpGPR Rm))
-      | _, _, _, _ => None
-      end
-
-
-    (* TODO: AND (immediate), 64-bit:
+      | (WO~ opc1~opc0 ~ 0~1~0~1~0 ~ 0~0 ~ 0 ~ Rm4~Rm3~Rm2~Rm1~Rm0 ~ 0~0~0~0~0~0
+           ~ Rn4~Rn3~Rn2~Rn1~Rn0 ~ Rd4~Rd3~Rd2~Rd1~Rd0)%word =>
+        match decode_log_op opc1 opc0,
+              decode_reg Rm4 Rm3 Rm2 Rm1 Rm0,
+              decode_reg Rn4 Rn3 Rn2 Rn1 Rn0,
+              decode_reg Rd4 Rd3 Rd2 Rd1 Rd0 with
+        | Some op, Some Rm, Some Rn, Some Rd => Some (LogOp op Rd Rn (OpGPR Rm))
+        | _, _, _, _ => None
+        end
+      (* TODO: AND (immediate), 64-bit:
        [(sf=1) 00 100100 N immr imms Rn Rd] *)
-    (* FIXME: *)
-    | _ => None
-    end.
+      (* FIXME: *)
+      | _ => None
+      end.
+  End Decode.
 
   Definition  next_pc (pc : mem_loc) (a : ast) : list mem_loc := [pc + 4].
 End AArch64.
